concurrency/conclib.v
@@ -180,7 +180,6 @@ Proof.
   intros; eapply derives_exclusive, data_at_exclusive; eauto.
 Qed.
 
-
 Lemma func_ptr_pre : forall sig cc A P1 P2 Q p, (forall a, P1 a ≡ P2 a) ->
   func_ptr (NDmk_funspec sig cc A P1 Q) p ⊢ func_ptr (NDmk_funspec sig cc A P2 Q) p.
 Proof.
