floyd/base2.v
@@ -55,7 +55,7 @@ Context `{!heapGS Σ}.
 
 Definition vacuous_funspec (fd: Clight.fundef): funspec :=
    NDmk_funspec (typesig_of_funsig (funsig_of_fundef fd)) (cc_of_fundef fd) 
-   (Impossible) (fun _ _ => False) (fun _ _ => False).
+   (Impossible) (fun _ => argsassert_of (fun _ => False)) (fun _ => postassert_of (fun _ => False)).
 
 
 Fixpoint augment_funspecs_new' (fds: list (ident * Clight.fundef)) (G: Maps.PTree.t funspec) : option funspecs :=
