veric/mpred.v
@@ -434,8 +434,6 @@ Context `{!heapGS Σ} `{!envGS Σ}.
 
 (* funspecs on mpreds *)
 Definition funspec := funspec_ mpred mpred.
-Definition NDmk_funspec (sig : typesig) (cc : calling_convention) A (P : A -> (genviron * list val) -> mpred) (Q : A -> option val -> mpred) : funspec :=
-  mk_funspec sig cc (ConstType A) (λne a, ⊤) (λne (a : leibnizO A), (P a) : _ -d> mpred) (λne (a : leibnizO A), (Q a) : _ -d> mpred).
 
 Definition funspec_unfold (f : funspec) : laterO funspec := Next f.
 
